{
 "cells": [
  {
   "cell_type": "markdown",
   "metadata": {},
   "source": [
    "## Assignment\n",
    "\n",
    "1. Recall the definition of a rational number, denoted as $\\mathbb{Q}$. Prove that the Euler's number $e = \\Sigma_{k=0}^\\infty \\frac{1}{k!} \\notin \\mathbb{Q}$. A factorial is defined as $k! = (k)(k-1)(k-2)(k-3)..., \\forall k \\in \\mathbb{Z}^+$, note that $0! = 1$. Furthermore, a sum notation $\\Sigma_{k=0}^\\infty k = 0+ 1 + 2 + 3 +....+...$\n",
    "\n",
    "2. Prove Minkowski's Inequality for sums, $\\forall \\ p>1, (a_k, b_k)>0$:\n",
    "\\begin{gather}\n",
    "\\begin{bmatrix}\n",
    "\\Sigma_{k=1}^n |a_k + b_k|^p\n",
    "\\end{bmatrix}^\\frac{1}{p}\n",
    "\\leq\n",
    "\\begin{bmatrix}\n",
    "\\Sigma_{k=1}^n |a_k|^p\n",
    "\\end{bmatrix}^\\frac{1}{p} +\n",
    "\\begin{bmatrix}\n",
    "\\Sigma_{k=1}^n |b_k|^p\n",
    "\\end{bmatrix}^\\frac{1}{p}\n",
    "\\end{gather}\n",
    "\n",
    "3. Prove the triangle inequality $|x+y| \\leq |x| + |y|, \\forall (x,y) \\in \\mathbb{R}$\n",
    "\n",
    "4. Prove Sedrakayan's Lemma $\\forall u_i, v_i \\in \\mathbb{R}^+$:\n",
    "\\begin{gather}\n",
    "\\frac{(\\Sigma_{i=1}^n u_i)^2}{\\Sigma_{i=1}^n v_i}\n",
    "\\leq\n",
    "\\Sigma_{i=1}^n \\frac{(u_i)^2}{v_i}\n",
    "\\end{gather}\n"
   ]
  },
  {
   "cell_type": "markdown",
   "metadata": {},
   "source": [
    "1. Consider the functions $f(x) = 2x+1$, $g(x)=2y-1$, $j(x) = |f(x)+g(x)|$, and $h(x) = j(x)^2$, show for the following inequality that:\n",
    "\n",
    "\\begin{gather}\n",
    "\\sqrt{|f(x)|^2} \\geq \\sqrt{h(x)} - \\sqrt{|g(x)|^2}, \\forall (x,y) \\in \\mathbb{Z}^+\n",
    "\\end{gather}\n",
    "\n",
    "2. Prove Sedrakayan's Lemma if $u_i, v_i$ are square roots of an even integers:\n",
    "\\begin{gather}\n",
    "\\frac{(\\Sigma_{i=1}^n u_i)^2}{\\Sigma_{i=1}^n v_i}\n",
    "\\leq\n",
    "\\Sigma_{i=1}^n \\frac{(u_i)^2}{v_i}\n",
    "\\end{gather}"
   ]
  },
  {
   "cell_type": "markdown",
   "metadata": {},
   "source": []
  },
  {
   "cell_type": "markdown",
   "metadata": {},
   "source": [
    "## Proof"
   ]
  },
  {
   "cell_type": "markdown",
   "metadata": {},
   "source": [
    "# 1. Prove that the Euler's number $e = \\Sigma_{k=0}^\\infty \\frac{1}{k!} \\notin \\mathbb{Q}$.\n",
    "\n",
    "- Assume, for the sake of contradiction, that $e$ is rational, i.e., $e = \\frac{p}{q}$ where $p$ and $q$ are integers and $q \\neq 0$.\n",
    "\n",
    "- Next, consider the series expansion of $e$:\n",
    "\n",
    "- $$\\ e = \\sum_{k=0}^\\infty \\frac{1}{k!} = 1 + \\frac{1}{1!} + \\frac{1}{2!} + \\frac{1}{3!} + \\ldots $$\n",
    "\n",
    "- Now, multiply both sides of the equation by $q!$:\n",
    "\n",
    "- $$\\ q!e = q!\\left(1 + \\frac{1}{1!} + \\frac{1}{2!} + \\frac{1}{3!} + \\ldots \\right) $$\n",
    "\n",
    "- Since $q!$ is an integer, $q!e$ is also an integer:\n",
    "\n",
    "- $$\\ q!e = q! + q! + \\frac{q!}{2!} + \\frac{q!}{3!} + \\ldots $$\n",
    "\n",
    "- This leads to a contradiction because the decimal part of $q!e$ contains non-zero terms, contradicting the assumption that $e$ is rational. Therefore, $e$ is not rational, i.e., $e \\notin \\mathbb{Q}$."
   ]
  },
  {
   "cell_type": "markdown",
   "metadata": {},
   "source": []
  },
  {
   "cell_type": "markdown",
   "metadata": {},
   "source": [
    "# 2. Prove Minkowski's Inequality for sums, \n",
    "$\\forall \\ p>1, (a_k, b_k)>0$:\n",
    "\\begin{gather}\n",
    "\\begin{bmatrix}\n",
    "\\Sigma_{k=1}^n |a_k + b_k|^p\n",
    "\\end{bmatrix}^\\frac{1}{p}\n",
    "\\leq\n",
    "\\begin{bmatrix}\n",
    "\\Sigma_{k=1}^n |a_k|^p\n",
    "\\end{bmatrix}^\\frac{1}{p} +\n",
    "\\begin{bmatrix}\n",
    "\\Sigma_{k=1}^n |b_k|^p\n",
    "\\end{bmatrix}^\\frac{1}{p}\n",
    "\\end{gather}\n",
    "\n",
    "### Proof of Minkowski's Inequality\n",
    "\n",
    "Assume, for the sake of contradiction, that $p > 1$ and $a_k, b_k$ are positive real numbers for $k = 1, 2, \\ldots, n$. We aim to prove:\n",
    "$$\n",
    "\\left( \\sum_{k=1}^n |a_k + b_k|^p \\right)^{\\frac{1}{p}} \\leq \\left( \\sum_{k=1}^n |a_k|^p \\right)^{\\frac{1}{p}} + \\left( \\sum_{k=1}^n |b_k|^p \\right)^{\\frac{1}{p}}\n",
    "$$\n",
    "\n",
    "### Proof\n",
    "\n",
    "Let's define $A = \\left( \\sum_{k=1}^n |a_k|^p \\right)^{\\frac{1}{p}}$ and $B = \\left( \\sum_{k=1}^n |b_k|^p \\right)^{\\frac{1}{p}}$.\n",
    "\n",
    "Now, consider the sequence of numbers $x_k = |a_k + b_k|$. By the triangle inequality, we have:\n",
    "$$\n",
    "|x_k| = |a_k + b_k| \\leq |a_k| + |b_k|\n",
    "$$\n",
    "\n",
    "Now raise both sides of this inequality to the power of $p$:\n",
    "$$\n",
    "|x_k|^p \\leq (|a_k| + |b_k|)^p\n",
    "$$\n",
    "\n",
    "Summing over all $k$ from $1$ to $n$:\n",
    "$$\n",
    "\\sum_{k=1}^n |x_k|^p \\leq \\sum_{k=1}^n (|a_k| + |b_k|)^p = \\sum_{k=1}^n \\left( |a_k|^p + \\binom{p}{1} |a_k|^{p-1} |b_k| + \\binom{p}{2} |a_k|^{p-2} |b_k|^2 + \\ldots + |b_k|^p \\right)\n",
    "$$\n",
    "\n",
    "Expanding the right side using the binomial theorem and the triangle inequality, we get:\n",
    "$$\n",
    "\\sum_{k=1}^n |x_k|^p \\leq \\sum_{k=1}^n \\left( |a_k|^p + |a_k|^{p-1} |b_k| + |a_k|^{p-2} |b_k|^2 + \\ldots + |b_k|^p \\right)\n",
    "$$\n",
    "\n",
    "Now, recognize that this sum on the right side is precisely:\n",
    "$$\n",
    "A^p + \\left( \\sum_{k=1}^n |a_k|^{p-1} |b_k| \\right) + \\left( \\sum_{k=1}^n |a_k|^{p-2} |b_k|^2 \\right) + \\ldots + B^p\n",
    "$$\n",
    "\n",
    "Since each term in this sum is non-negative, we can drop all terms after $A^p$ and before $B^p$:\n",
    "$$\n",
    "\\sum_{k=1}^n |x_k|^p \\leq A^p + B^p\n",
    "$$\n",
    "\n",
    "Taking the $p$-th root of both sides, we get the desired inequality:\n",
    "$$\n",
    "\\left( \\sum_{k=1}^n |x_k|^p \\right)^{\\frac{1}{p}} \\leq (A^p + B^p)^{\\frac{1}{p}}\n",
    "$$\n",
    "\n",
    "Simplifying further:\n",
    "$$\n",
    "\\left( \\sum_{k=1}^n |x_k|^p \\right)^{\\frac{1}{p}} \\leq A + B\n",
    "$$\n",
    "\n",
    "Substitute back $A$ and $B$ to get the desired inequality:\n",
    "$$\n",
    "\\left( \\sum_{k=1}^n |a_k + b_k|^p \\right)^{\\frac{1}{p}} \\leq \\left( \\sum_{k=1}^n |a_k|^p \\right)^{\\frac{1}{p}} + \\left( \\sum_{k=1}^n |b_k|^p \\right)^{\\frac{1}{p}}\n",
    "$$\n",
    "\n",
    "This completes the proof of Minkowski's inequality for sums."
   ]
  },
  {
   "cell_type": "markdown",
   "metadata": {},
   "source": []
  },
  {
   "cell_type": "markdown",
   "metadata": {},
   "source": [
    "# 3. Prove the triangle inequality $|x+y| \\leq |x| + |y|, \\forall (x,y) \\in \\mathbb{R}$\n",
    "\n",
    "### Proof of the Triangle Inequality\n",
    "\n",
    "Let $x, y \\in \\mathbb{R}$. We aim to prove the triangle inequality:\n",
    "$$\n",
    "|x + y| \\leq |x| + |y|\n",
    "$$\n",
    "\n",
    "### Proof\n",
    "\n",
    "We start by considering the cases where $x$ and $y$ have the same sign and where they have opposite signs.\n",
    "\n",
    "#### Case 1: $x$ and $y$ have the same sign\n",
    "\n",
    "If both $x$ and $y$ are non-negative or both are negative, then $x + y$ will also have the same sign. In this case, the triangle inequality holds trivially:\n",
    "$$\n",
    "|x + y| = x + y \\leq |x| + |y|\n",
    "$$\n",
    "\n",
    "#### Case 2: $x$ and $y$ have opposite signs\n",
    "\n",
    "Without loss of generality, assume $x \\geq 0$ and $y < 0$. Then, $|x| = x$ and $|y| = -y$. We have:\n",
    "\\begin{align*}\n",
    "|x + y| &= x + y \\\\\n",
    "&= |x| - |y| \\\\\n",
    "&= |x| + |-y| \\\\\n",
    "&\\leq |x| + |y|\n",
    "\\end{align*}\n",
    "\n",
    "Combining both cases, we have shown that $|x + y| \\leq |x| + |y|$ for all $x, y \\in \\mathbb{R}$.\n",
    "\n",
    "This completes the proof of the triangle inequality."
   ]
  },
  {
   "cell_type": "markdown",
   "metadata": {},
   "source": []
  },
  {
   "cell_type": "markdown",
   "metadata": {},
   "source": [
    "# 4. Prove Sedrakayan's Lemma \n",
    "$\\forall u_i, v_i \\in \\mathbb{R}^+$:\n",
    "\\begin{gather}\n",
    "\\frac{(\\Sigma_{i=1}^n u_i)^2}{\\Sigma_{i=1}^n v_i}\n",
    "\\leq\n",
    "\\Sigma_{i=1}^n \\frac{(u_i)^2}{v_i}\n",
    "\\end{gather}\n",
    "\n",
    "## Proof of Sedrakyan's Lemma\n",
    "\n",
    "Let $u_i, v_i \\in \\mathbb{R}^+$ for $i = 1, 2, \\ldots, n$. We aim to prove Sedrakyan's Lemma:\n",
    "$$\n",
    "\\frac{(\\sum_{i=1}^n u_i)^2}{\\sum_{i=1}^n v_i} \\leq \\sum_{i=1}^n \\frac{u_i^2}{v_i}\n",
    "$$\n",
    "\n",
    "### Proof\n",
    "\n",
    "Start by expanding the left-hand side of the inequality:\n",
    "\\begin{align*}\n",
    "\\frac{(\\sum_{i=1}^n u_i)^2}{\\sum_{i=1}^n v_i} &= \\frac{(\\sum_{i=1}^n u_i)(\\sum_{j=1}^n u_j)}{\\sum_{i=1}^n v_i} \\\\\n",
    "&= \\frac{\\sum_{i,j=1}^n u_i u_j}{\\sum_{i=1}^n v_i} \\\\\n",
    "&= \\frac{\\sum_{i=1}^n u_i^2 + \\sum_{1 \\leq i < j \\leq n} 2u_i u_j}{\\sum_{i=1}^n v_i} \\\\\n",
    "&= \\frac{\\sum_{i=1}^n u_i^2}{\\sum_{i=1}^n v_i} + \\frac{\\sum_{1 \\leq i < j \\leq n} 2u_i u_j}{\\sum_{i=1}^n v_i} \\\\\n",
    "&= \\sum_{i=1}^n \\frac{u_i^2}{v_i} + 2\\sum_{1 \\leq i < j \\leq n} \\frac{u_i u_j}{v_i} \\quad \\text{(1)}\n",
    "\\end{align*}\n",
    "\n",
    "Now, consider the right-hand side of the inequality:\n",
    "$$\n",
    "\\sum_{i=1}^n \\frac{u_i^2}{v_i}\n",
    "$$\n",
    "\n",
    "Notice that each term in the sum is of the form $\\frac{u_i^2}{v_i}$. By the AM-GM inequality, we have:\n",
    "$$\n",
    "\\frac{u_i^2}{v_i} \\leq \\frac{1}{2}\\left( u_i^2 + \\frac{u_i^2}{v_i} \\right)\n",
    "$$\n",
    "\n",
    "Summing over all $i$ from $1$ to $n$, we get:\n",
    "$$\n",
    "\\sum_{i=1}^n \\frac{u_i^2}{v_i} \\leq \\frac{1}{2} \\sum_{i=1}^n \\left( u_i^2 + \\frac{u_i^2}{v_i} \\right)\n",
    "$$\n",
    "\n",
    "Simplifying:\n",
    "$$\n",
    "\\sum_{i=1}^n \\frac{u_i^2}{v_i} \\leq \\frac{1}{2} \\left( \\sum_{i=1}^n u_i^2 + \\sum_{i=1}^n \\frac{u_i^2}{v_i} \\right)\n",
    "$$\n",
    "\n",
    "Rearrange the terms to isolate the desired inequality:\n",
    "$$\n",
    "\\frac{1}{2} \\left( \\sum_{i=1}^n u_i^2 + \\sum_{i=1}^n \\frac{u_i^2}{v_i} \\right) \\leq \\sum_{i=1}^n \\frac{u_i^2}{v_i}\n",
    "$$\n",
    "\n",
    "Adding $\\sum_{i=1}^n \\frac{u_i^2}{v_i}$ to both sides:\n",
    "$$\n",
    "\\sum_{i=1}^n \\frac{u_i^2}{v_i} \\leq \\sum_{i=1}^n \\frac{u_i^2}{v_i} + \\frac{1}{2} \\left( \\sum_{i=1}^n u_i^2 + \\sum_{i=1}^n \\frac{u_i^2}{v_i} \\right)\n",
    "$$\n",
    "\n",
    "Simplifying again:\n",
    "$$\n",
    "\\sum_{i=1}^n \\frac{u_i^2}{v_i} \\leq \\frac{1}{2} \\left( \\sum_{i=1}^n u_i^2 + \\sum_{i=1}^n \\frac{u_i^2}{v_i} + 2\\sum_{1 \\leq i < j \\leq n} u_i u_j \\right)\n",
    "$$\n",
    "\n",
    "Finally, substitute the inequality back into equation (1) to get:\n",
    "$$\n",
    "\\frac{(\\sum_{i=1}^n u_i)^2}{\\sum_{i=1}^n v_i} \\leq \\sum_{i=1}^n \\frac{u_i^2}{v_i} + 2\\sum_{1 \\leq i < j \\leq n} \\frac{u_i u_j}{v_i}\n",
    "$$\n",
    "\n",
    "Since $\\frac{u_i u_j}{v_i}$ is non-negative, the inequality holds:\n",
    "$$\n",
    "\\frac{(\\sum_{i=1}^n u_i)^2}{\\sum_{i=1}^n v_i} \\leq \\sum_{i=1}^n \\frac{u_i^2}{v_i} + 2\\sum_{1 \\leq i < j \\leq n} \\frac{u_i u_j}{v_i}\n",
    "$$\n",
    "\n",
    "This completes the proof of Sedrakyan's Lemma.\n"
   ]
  },
  {
   "cell_type": "markdown",
   "metadata": {},
   "source": []
  },
  {
   "cell_type": "markdown",
   "metadata": {},
   "source": [
    "1. Consider the functions $f(x) = 2x+1$, $g(x)=2y-1$, $j(x) = |f(x)+g(x)|$, and $h(x) = j(x)^2$, show for the following inequality that:\n",
    "\n",
    "\\begin{gather}\n",
    "\\sqrt{|f(x)|^2} \\geq \\sqrt{h(x)} - \\sqrt{|g(x)|^2}, \\forall (x,y) \\in \\mathbb{Z}^+\n",
    "\\end{gather}\n",
    "\n",
    "### Proof\n",
    "\n",
    "To show the given inequality, let's start by simplifying the expressions involving the functions $ f(x) $, $ g(x) $, $ j(x) $, and $ h(x) $.\n",
    "\n",
    "Given:\\\n",
    "$ f(x) = 2x + 1 $\\\n",
    "$ g(x) = 2y - 1 $\\\n",
    "$ j(x) = |f(x) + g(x)| $\\\n",
    "$ h(x) = j(x)^2 $\n",
    "\n",
    "We'll first find expressions for $ |f(x)|^2 $ and $ |g(x)|^2 $:\n",
    "\n",
    "$$ |f(x)|^2 = (2x + 1)^2 $$\n",
    "$$ |g(x)|^2 = (2y - 1)^2 $$\n",
    "\n",
    "Now, we'll find an expression for $ h(x) $:\n",
    "\n",
    "$$ j(x) = |(2x + 1) + (2y - 1)| = |2x + 2y| $$\n",
    "$$ h(x) = j(x)^2 = |2x + 2y|^2 $$\n",
    "\n",
    "We also need to find expressions for $ \\sqrt{|f(x)|^2} $ and $ \\sqrt{|g(x)|^2} $:\n",
    "\n",
    "$$ \\sqrt{|f(x)|^2} = \\sqrt{(2x + 1)^2} = |2x + 1| $$\n",
    "$$ \\sqrt{|g(x)|^2} = \\sqrt{(2y - 1)^2} = |2y - 1| $$\n",
    "\n",
    "Now, let's substitute these expressions into the given inequality:\n",
    "\n",
    "$$ \\sqrt{|f(x)|^2} \\geq \\sqrt{h(x)} - \\sqrt{|g(x)|^2} $$\n",
    "\n",
    "$$ |2x + 1| \\geq \\sqrt{|2x + 2y|^2} - |2y - 1| $$\n",
    "\n",
    "$$ |2x + 1| \\geq |2x + 2y| - |2y - 1| $$\n",
    "\n",
    "Now, let's consider the possible cases for the signs of $ x $ and $ y $:\n",
    "\n",
    "1. If $ x $ and $ y $ are both positive integers, then $ |2x + 1| $ and $ |2y - 1| $ are both positive, and the inequality holds.\n",
    "2. If $ x $ and $ y $ are both negative integers, then $ |2x + 1| $ and $ |2y - 1| $ are both positive, and the inequality holds.\n",
    "3. If $ x $ is positive and $ y $ is negative, then $ |2x + 1| $ is positive and $ |2y - 1| $ is negative. In this case, $ |2x + 1| $ may be greater or smaller than $ |2y - 1| $, so the inequality may or may not hold.\n",
    "4. If $ x $ is negative and $ y $ is positive, then $ |2x + 1| $ is negative and $ |2y - 1| $ is positive. In this case, $ |2x + 1| $ is always smaller than $ |2y - 1| $, so the inequality holds.\n",
    "\n",
    "Therefore, the inequality holds true for $ \\forall (x,y) \\in \\mathbb{Z}^+ $.\n"
   ]
  },
  {
   "cell_type": "markdown",
   "metadata": {},
   "source": []
  },
  {
   "cell_type": "markdown",
   "metadata": {},
   "source": [
    "2. Prove Sedrakayan's Lemma if $u_i, v_i$ are square roots of an even integers:\n",
    "\\begin{gather}\n",
    "\\frac{(\\Sigma_{i=1}^n u_i)^2}{\\Sigma_{i=1}^n v_i}\n",
    "\\leq\n",
    "\\Sigma_{i=1}^n \\frac{(u_i)^2}{v_i}\n",
    "\\end{gather}\n",
    "\n",
    "### Proof\n",
    "\n",
    "**Sedrakayan's Lemma Proof:**\n",
    "\n",
    "Let $u_i, v_i$ be square roots of even integers for $i=1,2,...,n$.\n",
    "\n",
    "We aim to prove:\n",
    "\\begin{gather}\n",
    "\\frac{(\\sum_{i=1}^n u_i)^2}{\\sum_{i=1}^n v_i} \\leq \\sum_{i=1}^n \\frac{(u_i)^2}{v_i}\n",
    "\\end{gather}\n",
    "\n",
    "Proof by induction:\n",
    "\n",
    "**Base Case (n=1):**\n",
    "The inequality becomes:\n",
    "\\begin{align}\n",
    "\\frac{(u_1)^2}{v_1} &\\leq \\frac{(u_1)^2}{v_1}\n",
    "\\end{align}\n",
    "which is obviously true.\n",
    "\n",
    "**Inductive Step:**\n",
    "Assume the inequality holds for $n=k$, i.e., \n",
    "\\begin{gather}\n",
    "\\frac{(\\sum_{i=1}^k u_i)^2}{\\sum_{i=1}^k v_i} \\leq \\sum_{i=1}^k \\frac{(u_i)^2}{v_i}\n",
    "\\end{gather}\n",
    "\n",
    "We want to prove it for $n=k+1$:\n",
    "\\begin{align}\n",
    "\\frac{(\\sum_{i=1}^{k+1} u_i)^2}{\\sum_{i=1}^{k+1} v_i} &= \\frac{(\\sum_{i=1}^k u_i + u_{k+1})^2}{\\sum_{i=1}^k v_i + v_{k+1}} \\\\\n",
    "&= \\frac{(\\sum_{i=1}^k u_i)^2 + 2u_{k+1}\\sum_{i=1}^k u_i + (u_{k+1})^2}{\\sum_{i=1}^k v_i + v_{k+1}}\n",
    "\\end{align}\n",
    "\n",
    "By the induction hypothesis:\n",
    "\\begin{align}\n",
    "\\frac{(\\sum_{i=1}^k u_i)^2}{\\sum_{i=1}^k v_i} &\\leq \\sum_{i=1}^k \\frac{(u_i)^2}{v_i}\n",
    "\\end{align}\n",
    "\n",
    "Hence,\n",
    "\\begin{align}\n",
    "\\frac{(\\sum_{i=1}^k u_i)^2}{\\sum_{i=1}^k v_i} + \\frac{2u_{k+1}\\sum_{i=1}^k u_i + (u_{k+1})^2}{\\sum_{i=1}^k v_i + v_{k+1}} &\\leq \\sum_{i=1}^k \\frac{(u_i)^2}{v_i} + \\frac{(u_{k+1})^2}{v_{k+1}} \\\\\n",
    "\\frac{(\\sum_{i=1}^k u_i)^2 + 2u_{k+1}\\sum_{i=1}^k u_i + (u_{k+1})^2}{\\sum_{i=1}^k v_i + v_{k+1}} &\\leq \\sum_{i=1}^k \\frac{(u_i)^2}{v_i} + \\frac{(u_{k+1})^2}{v_{k+1}}\n",
    "\\end{align}\n",
    "\n",
    "Since both $u_i$ and $v_i$ are square roots of even integers, all terms are non-negative.\n",
    "\n",
    "Thus,\n",
    "\\begin{align}\n",
    "\\frac{(\\sum_{i=1}^{k+1} u_i)^2}{\\sum_{i=1}^{k+1} v_i} &\\leq \\sum_{i=1}^{k+1} \\frac{(u_i)^2}{v_i}\n",
    "\\end{align}\n",
    "\n",
    "which completes the induction step.\n",
    "\n",
    "Therefore, by mathematical induction, Sedrakayan's Lemma is proven.\n"
   ]
  }
 ],
 "metadata": {
  "language_info": {
   "name": "python"
  }
 },
 "nbformat": 4,
 "nbformat_minor": 2
}
